src/lib/respectful9.v
@@ -1,0 +1,232 @@
+Require Import paco9.
+Require Import sflib.
+
+Set Implicit Arguments.
+
+Section Respectful9.
+  Variable T0: Type.
+  Variable T1: forall (x0: @T0), Type.
+  Variable T2: forall (x0: @T0) (x1: @T1 x0), Type.
+  Variable T3: forall (x0: @T0) (x1: @T1 x0) (x2: @T2 x0 x1), Type.
+  Variable T4: forall (x0: @T0) (x1: @T1 x0) (x2: @T2 x0 x1) (x3: @T3 x0 x1 x2), Type.
+  Variable T5: forall (x0: @T0) (x1: @T1 x0) (x2: @T2 x0 x1) (x3: @T3 x0 x1 x2) (x4: @T4 x0 x1 x2 x3), Type.
+  Variable T6: forall (x0: @T0) (x1: @T1 x0) (x2: @T2 x0 x1) (x3: @T3 x0 x1 x2) (x4: @T4 x0 x1 x2 x3) (x5: @T5 x0 x1 x2 x3 x4), Type.
+  Variable T7: forall (x0: @T0) (x1: @T1 x0) (x2: @T2 x0 x1) (x3: @T3 x0 x1 x2) (x4: @T4 x0 x1 x2 x3) (x5: @T5 x0 x1 x2 x3 x4) (x6: @T6 x0 x1 x2 x3 x4 x5), Type.
+  Variable T8: forall (x0: @T0) (x1: @T1 x0) (x2: @T2 x0 x1) (x3: @T3 x0 x1 x2) (x4: @T4 x0 x1 x2 x3) (x5: @T5 x0 x1 x2 x3 x4) (x6: @T6 x0 x1 x2 x3 x4 x5) (x7: @T7 x0 x1 x2 x3 x4 x5 x6), Type.
+  Definition rel := rel9 T0 T1 T2 T3 T4 T5 T6 T7 T8.
+
+  Variable gf: rel -> rel.
+  Hypothesis gf_mon: monotone9 gf.
+
+  Inductive sound9 (clo: rel -> rel): Prop :=
+  | sound9_intro
+      (MON: monotone9 clo)
+      (SOUND:
+         forall r (PFIX: r <9= gf (clo r)),
+           r <9= paco9 gf bot9)
+  .
+  Hint Constructors sound9.
+
+  Structure respectful9 (clo: rel -> rel) : Prop :=
+  | respectful9_intro
+      (MON: monotone9 clo)
+      (RESPECTFUL:
+         forall l r (LE: l <9= r) (GF: l <9= gf r),
+           clo l <9= gf (clo r)).
+  Hint Constructors respectful9.
+
+  Inductive grespectful9 (r: rel) e1 e2 e3 e4 e5 e6 e7 e8 e9: Prop :=
+  | grespectful9_intro
+      clo
+      (RES: respectful9 clo)
+      (CLO: clo r e1 e2 e3 e4 e5 e6 e7 e8 e9)
+  .
+  Hint Constructors grespectful9.
+
+  Lemma gfclo9_mon: forall clo, sound9 clo -> monotone9 (gf <*> clo).
+  Proof. intros; destruct H; eauto using gf_mon. Qed.
+  Hint Resolve gfclo9_mon : paco.
+
+  Lemma sound9_is_gf: forall clo (UPTO: sound9 clo),
+      paco9 (gf <*> clo) bot9 <9= paco9 gf bot9.
+  Proof.
+    i. punfold PR. edestruct UPTO.
+    eapply (SOUND (paco9 (gf <*> clo) bot9)); eauto.
+    i. punfold PR0.
+    eapply (gfclo9_mon UPTO); eauto.
+    intros. destruct PR1; eauto. done.
+  Qed.
+
+  Lemma respectful9_is_sound9: respectful9 <1= sound9.
+  Proof.
+    intro clo.
+    set (rclo := fix rclo clo n (r: rel) :=
+           match n with
+           | 0 => r
+           | S n' => rclo clo n' r \9/ clo (rclo clo n' r)
+           end).
+    i. destruct PR. econs; eauto.
+    i. set (rr e1 e2 e3 e4 e5 e6 e7 e8 e9 := exists n, rclo clo n r e1 e2 e3 e4 e5 e6 e7 e8 e9).
+    assert (rr x0 x1 x2 x3 x4 x5 x6 x7 x8) by (exists 0; eauto); clear PR.
+    cut (forall n, rclo clo n r <9= gf (rclo clo (S n) r)).
+    { intro X; revert x0 x1 x2 x3 x4 x5 x6 x7 x8 H; pcofix CIH; i.
+      unfold rr in *; des; eauto 10 using gf_mon. }
+    induction n; i; [by s; eauto using gf_mon|].
+    ss; des; [by eauto using gf_mon|].
+    eapply gf_mon; [eapply RESPECTFUL; [|apply IHn|]|]; inst; s; eauto.
+  Qed.
+
+  Lemma respectful9_compose
+        clo1 clo2
+        (RES1: respectful9 clo1)
+        (RES2: respectful9 clo2):
+    respectful9 (clo1 <*> clo2).
+  Proof.
+    i. destruct RES1, RES2.
+    econs.
+    - ii. eapply MON; eauto.
+    - i. eapply RESPECTFUL; [| |apply PR].
+      + i. eapply MON0; eauto.
+      + i. eapply RESPECTFUL0; eauto.
+  Qed.
+
+  Lemma grespectful9_respectful9: respectful9 grespectful9.
+  Proof.
+    econs; ii.
+    - destructs IN RES; exists clo; eauto.
+    - destructs PR RES; eapply gf_mon with (r:=clo r); eauto.
+  Qed.
+
+  Lemma gfgres9_mon: monotone9 (gf <*> grespectful9).
+  Proof.
+    destruct grespectful9_respectful9; eauto using gf_mon.
+  Qed.
+  Hint Resolve gfgres9_mon : paco.
+
+  Lemma grespectful9_greatest: forall clo (RES: respectful9 clo), clo <10= grespectful9.
+  Proof.
+    eauto.
+  Qed.
+
+  Lemma grespectful9_incl: forall r, r <9= grespectful9 r.
+  Proof.
+    i; eexists (fun x => x); eauto.
+  Qed.
+  Hint Resolve grespectful9_incl.
+
+  Lemma grespectful9_compose: forall clo (RES: respectful9 clo) r,
+      clo (grespectful9 r) <9= grespectful9 r.
+  Proof.
+    i; eapply grespectful9_greatest with (clo := clo <*> grespectful9);
+      eauto using respectful9_compose, grespectful9_respectful9.
+  Qed.
+
+  Lemma grespectful9_incl_rev: forall r,
+      grespectful9 (paco9 (gf <*> grespectful9) r) <9= paco9 (gf <*> grespectful9) r.
+  Proof.
+    intro r; pcofix CIH; i; pfold.
+    eapply gf_mon, grespectful9_compose, grespectful9_respectful9.
+    destruct grespectful9_respectful9; eapply RESPECTFUL, PR; i; [by eauto using grespectful9_incl|].
+    punfold PR0.
+      by eapply gfgres9_mon; eauto; i; destruct PR1; eauto.
+  Qed.
+
+  Inductive rclo9 clo (r: rel): rel :=
+  | rclo9_incl
+      e1 e2 e3 e4 e5 e6 e7 e8 e9
+      (R: r e1 e2 e3 e4 e5 e6 e7 e8 e9):
+      @rclo9 clo r e1 e2 e3 e4 e5 e6 e7 e8 e9
+  | rclo9_step'
+      r' e1 e2 e3 e4 e5 e6 e7 e8 e9
+      (R': r' <9= rclo9 clo r)
+      (CLOR':clo r' e1 e2 e3 e4 e5 e6 e7 e8 e9):
+      @rclo9 clo r e1 e2 e3 e4 e5 e6 e7 e8 e9
+  .
+
+  Lemma rclo9_mon clo:
+    monotone9 (rclo9 clo).
+  Proof.
+    ii. induction IN.
+    - econs 1. auto.
+    - econs 2; eauto.
+  Qed.
+  Hint Resolve rclo9_mon: paco.
+
+  Lemma rclo9_base
+        clo
+        (MON: monotone9 clo):
+    clo <10= rclo9 clo.
+  Proof.
+    s. i. econs 2; eauto.
+    eapply MON; eauto. i.
+    econs 1. eauto.
+  Qed.
+
+  Lemma rclo9_step
+        (clo: rel -> rel) r:
+    clo (rclo9 clo r) <9= rclo9 clo r.
+  Proof.
+    i. econs 2; eauto.
+  Qed.
+
+  Lemma rclo9_rclo9
+        clo r
+        (MON: monotone9 clo):
+    rclo9 clo (rclo9 clo r) <9= rclo9 clo r.
+  Proof.
+    i. induction PR; eauto.
+    econs 2; eauto.
+  Qed.
+
+  Structure weak_respectful9 (clo: rel -> rel) : Prop :=
+  | weak_respectful9_intro
+      (MON: monotone9 clo)
+      (RESPECTFUL:
+         forall l r (LE: l <9= r) (GF: l <9= gf r),
+           clo l <9= gf (rclo9 clo r)).
+  Hint Constructors weak_respectful9.
+
+  Lemma weak_respectful9_respectful9
+        clo (RES: weak_respectful9 clo):
+    respectful9 (rclo9 clo).
+  Proof.
+    inv RES. econs; eauto with paco. i.
+    induction PR; i.
+    - eapply gf_mon; eauto. i.
+      apply rclo9_incl. auto.
+    - exploit RESPECTFUL; [|apply H|apply CLOR'|].
+      + i. eapply rclo9_mon; eauto.
+      + i. eapply gf_mon; eauto.
+        apply rclo9_rclo9; auto.
+  Qed.
+
+  Lemma upto9_init:
+      paco9 (gf <*> grespectful9) bot9 <9= paco9 gf bot9.
+  Proof.
+    apply sound9_is_gf; eauto.
+    apply respectful9_is_sound9.
+    apply grespectful9_respectful9.
+  Qed.
+
+  Lemma upto9_final:
+    paco9 gf <10= paco9 (gf <*> grespectful9).
+  Proof.
+    pcofix CIH. i. punfold PR. pfold.
+    eapply gf_mon; [|apply grespectful9_incl].
+    eapply gf_mon; eauto. right. des; auto.
+  Qed.
+
+  Lemma upto9_step
+        r clo (RES: weak_respectful9 clo):
+    clo (paco9 (gf <*> grespectful9) r) <9= paco9 (gf <*> grespectful9) r.
+  Proof.
+    i. apply grespectful9_incl_rev.
+    exploit weak_respectful9_respectful9; eauto. i.
+    eapply grespectful9_greatest; eauto.
+    apply rclo9_base; auto. inv RES. auto.
+  Qed.
+End Respectful9.
+
+Ltac pupto9_init := apply upto9_init; eauto with paco.
+Ltac pupto9_final := apply upto9_final; eauto with paco.
+Ltac pupto9 H := eapply upto9_step; [|exact H|]; eauto with paco.
